<?xml version="1.0"?>


<!DOCTYPE rdf:RDF [
    <!ENTITY owl "http://www.w3.org/2002/07/owl#" >
    <!ENTITY xsd "http://www.w3.org/2001/XMLSchema#" >
    <!ENTITY xml "http://www.w3.org/XML/1998/namespace" >
    <!ENTITY rdfs "http://www.w3.org/2000/01/rdf-schema#" >
    <!ENTITY rdf "http://www.w3.org/1999/02/22-rdf-syntax-ns#" >
]>


<rdf:RDF xmlns="https://w3id.org/associations/vocab#"
     xml:base="https://w3id.org/associations/vocab"
     xmlns:rdf="http://www.w3.org/1999/02/22-rdf-syntax-ns#"
     xmlns:owl="http://www.w3.org/2002/07/owl#"
     xmlns:xml="http://www.w3.org/XML/1998/namespace"
     xmlns:xsd="http://www.w3.org/2001/XMLSchema#"
     xmlns:rdfs="http://www.w3.org/2000/01/rdf-schema#">
    <owl:Ontology rdf:about="https://w3id.org/associations/vocab">
        <owl:versionInfo>1.0.0</owl:versionInfo>
        <owl:versionIRI rdf:resource="https://w3id.org/associations/vocab/1.0.0"/>
    </owl:Ontology>
    


    <!-- 
    ///////////////////////////////////////////////////////////////////////////////////////
    //
    // Object Properties
    //
    ///////////////////////////////////////////////////////////////////////////////////////
     -->

    


    <!-- https://w3id.org/associations/vocab#mappedTo -->

    <owl:ObjectProperty rdf:about="https://w3id.org/associations/vocab#mappedTo">
        <rdfs:label>mapped to</rdfs:label>
        <rdfs:comment>A mapping from an association in one dataset to an equivalent one in another.</rdfs:comment>
        <rdfs:range rdf:resource="https://w3id.org/associations/vocab#Association"/>
        <rdfs:domain rdf:resource="https://w3id.org/associations/vocab#Association"/>
    </owl:ObjectProperty>
    


    <!-- https://w3id.org/associations/vocab#response -->

    <owl:ObjectProperty rdf:about="https://w3id.org/associations/vocab#response">
        <rdfs:label>response</rdfs:label>
        <rdfs:comment>The response term of an association.</rdfs:comment>
        <rdfs:domain rdf:resource="https://w3id.org/associations/vocab#Association"/>
        <rdfs:range rdf:resource="https://w3id.org/associations/vocab#Term"/>
    </owl:ObjectProperty>
    


    <!-- https://w3id.org/associations/vocab#stimulus -->

    <owl:ObjectProperty rdf:about="https://w3id.org/associations/vocab#stimulus">
        <rdfs:label>stimulus</rdfs:label>
        <rdfs:comment>The stimulus term of an association.</rdfs:comment>
        <rdfs:domain rdf:resource="https://w3id.org/associations/vocab#Association"/>
        <rdfs:range rdf:resource="https://w3id.org/associations/vocab#Term"/>
    </owl:ObjectProperty>
    


    <!-- 
    ///////////////////////////////////////////////////////////////////////////////////////
    //
    // Data properties
    //
    ///////////////////////////////////////////////////////////////////////////////////////
     -->

    


    <!-- https://w3id.org/associations/vocab#count -->

    <owl:DatatypeProperty rdf:about="https://w3id.org/associations/vocab#count">
        <rdfs:label>count</rdfs:label>
        <rdfs:comment>The count how often this association occurred.</rdfs:comment>
        <rdfs:domain rdf:resource="https://w3id.org/associations/vocab#Association"/>
        <rdfs:range rdf:resource="&xsd;positiveInteger"/>
    </owl:DatatypeProperty>
    


    <!-- https://w3id.org/associations/vocab#frequency -->

    <owl:DatatypeProperty rdf:about="https://w3id.org/associations/vocab#frequency">
        <rdfs:label>frequency</rdfs:label>
        <rdfs:comment>The relative count of this association wrt. all associations of the stimulus.</rdfs:comment>
        <rdfs:domain rdf:resource="https://w3id.org/associations/vocab#Association"/>
        <rdfs:range>
            <rdfs:Datatype>
                <owl:onDatatype rdf:resource="&xsd;double"/>
                <owl:withRestrictions rdf:parseType="Collection">
                    <rdf:Description>
                        <xsd:minExclusive rdf:datatype="&xsd;double">0.0</xsd:minExclusive>
                    </rdf:Description>
                    <rdf:Description>
                        <xsd:maxInclusive rdf:datatype="&xsd;double">1.0</xsd:maxInclusive>
                    </rdf:Description>
                </owl:withRestrictions>
            </rdfs:Datatype>
        </rdfs:range>
    </owl:DatatypeProperty>
    


    <!-- 
    ///////////////////////////////////////////////////////////////////////////////////////
    //
    // Classes
    //
    ///////////////////////////////////////////////////////////////////////////////////////
     -->

    


    <!-- https://w3id.org/associations/vocab#Association -->

    <owl:Class rdf:about="https://w3id.org/associations/vocab#Association">
        <rdfs:label>Association</rdfs:label>
        <rdfs:comment>An association having a stimulus and a respone, a count and frequency.</rdfs:comment>
    </owl:Class>
    


    <!-- https://w3id.org/associations/vocab#Mapping -->

    <owl:Class rdf:about="https://w3id.org/associations/vocab#Mapping">
        <rdfs:label>Mapping</rdfs:label>
        <rdfs:comment>A mapping in the context of associations. If an association is an instance of this class it typically wasn&apos;t directly created on the dataset of the stimulus and response but was mapped to the entities from another dataset (see the mappedTo property).</rdfs:comment>
    </owl:Class>
    


    <!-- https://w3id.org/associations/vocab#Term -->

    <owl:Class rdf:about="https://w3id.org/associations/vocab#Term">
        <rdfs:label>Term</rdfs:label>
        <rdfs:comment>A class representing an association term that can either occur as stimulus or as response of an association.</rdfs:comment>
    </owl:Class>
    


    <!-- https://w3id.org/associations/vocab#VerifiedMapping -->

    <owl:Class rdf:about="https://w3id.org/associations/vocab#VerifiedMapping">
        <rdfs:label>VerifiedMapping</rdfs:label>
        <rdfs:subClassOf rdf:resource="https://w3id.org/associations/vocab#Mapping"/>
        <rdfs:comment>A mapping that has been manually verified.</rdfs:comment>
    </owl:Class>
</rdf:RDF>



<!-- Generated by the OWL API (version 3.5.1) http://owlapi.sourceforge.net -->

